@prefix schema: <http://schema.org/> .
@prefix pav: <http://purl.org/pav/> .
@prefix adms: <http://www.w3.org/ns/adms#> .
@prefix owl: <http://www.w3.org/2002/07/owl#> .
@prefix org: <http://www.w3.org/ns/org#> .
@prefix xls2rdf: <https://xls2rdf.sparna.fr/vocabulary#> .
@prefix xsd: <http://www.w3.org/2001/XMLSchema#> .
@prefix skosthes: <http://purl.org/iso25964/skos-thes#> .
@prefix rdfs: <http://www.w3.org/2000/01/rdf-schema#> .
@prefix idtype: <https://w3id.org/gofairus/vocs/train1/idtype-grna/> .
@prefix qb: <http://purl.org/linked-data/cube#> .
@prefix dct: <http://purl.org/dc/terms/> .
@prefix rdf: <http://www.w3.org/1999/02/22-rdf-syntax-ns#> .
@prefix doap: <http://usefulinc.com/ns/doap#> .
@prefix sh: <http://www.w3.org/ns/shacl#> .
@prefix dcat: <http://www.w3.org/ns/dcat#> .
@prefix euvoc: <http://publications.europa.eu/ontology/euvoc#> .
@prefix prov: <http://www.w3.org/ns/prov#> .
@prefix foaf: <http://xmlns.com/foaf/0.1/> .
@prefix dc: <http://purl.org/dc/elements/1.1/> .
@prefix skos: <http://www.w3.org/2004/02/skos/core#> .
@prefix skosxl: <http://www.w3.org/2008/05/skos-xl#> .

<https://w3id.org/gofairus/vocs/train1/idtype-grna> a skos:ConceptScheme;
  dct:title "Working identifier types vocabulary for Green Team A";
  skos:prefLabel "Working identifier types vocabulary for Green Team A";
  dct:description "This vocabulary contains the identifier components from the FDC-GDMT ontolgy (https://bioportal.bioontology.org/ontologies/FDC-GDMT) in BioPortal. It also serves as a training template for modifying an excel2rdf-formatted ontology, as described in excel2rdf.readthedocs.io. This is the vocabulary for Green Team A.";
  foaf:homepage <https://docs.google.com/document/d/130OKPxv9i7Vnej4JVLLotNFgwOrxt1hPeBcy78RC0rM>;
  dct:creator <https://orcid.org/0000-0001-6875-5360>;
  dct:conbtributor <https://orcid.org/0000-0001-8888-635X>;
  dct:rights <https://spdx.org/licenses/CC0-1.0>;
  dct:hasVersion "0.9.0";
  dct:created "2022-06-01T00:00:00+00:00"^^xsd:datetime;
  dct:modified "2025-06-08T16:32:00-07:00"^^xsd:datetime;
  skos:hasTopConcept idtype:identifiertype .

idtype:identifiertype a skos:Concept;
  skos:prefLabel "Identifier Type"@en;
  skos:definition "The type of internet identifier used for the resource. Note many of these identifier types are *not* IRIs."@en;
  skos:narrower idtype:ark, idtype:arxiv, idtype:bibcode, idtype:doi, idtype:ean13,
    idtype:eissn, idtype:handle, idtype:igsn, idtype:iri, idtype:isbn, idtype:issn, idtype:istc,
    idtype:lissn, idtype:lsid, idtype:pmid, idtype:purl, idtype:upc, idtype:uri, idtype:url,
    idtype:urn;
  skos:inScheme <https://w3id.org/gofairus/vocs/train1/idtype-grna>;
  skos:topConceptOf <https://w3id.org/gofairus/vocs/train1/idtype-grna> .

idtype:ark a skos:Concept;
  skos:prefLabel "ARK"@en;
  skos:definition "Archival Resource Key; URL designed to support long-term access to information objects. In general, ARK syntax is of the form (brackets indicate [optional] elements: [http://NMA/]ark:/NAAN/Name [Qualifier]"@en;
  skos:broader idtype:identifiertype;
  skos:inScheme <https://w3id.org/gofairus/vocs/train1/idtype-grna> .

idtype:arxiv a skos:Concept;
  skos:prefLabel "arXiv"@en;
  skos:definition "arXiv identifier; arXiv.org is a repository of preprints of scientific papers in the fields of mathematics, physics, astronomy, computer science, quantitative biology, statistics, and quantitative finance."@en;
  skos:broader idtype:identifiertype;
  skos:inScheme <https://w3id.org/gofairus/vocs/train1/idtype-grna> .

idtype:bibcode a skos:Concept;
  skos:prefLabel "bibcode"@en;
  skos:definition "Astrophysics Data System bibliographic codes; a standardized 19 character identifier according to the syntax yyyyjjjjjvvvvmppppa. See http://info- uri.info/registry/OAIHandler?verb=GetRecord&metadataPrefix=reg&identifier=info:bibcode/"@en;
  skos:broader idtype:identifiertype;
  skos:inScheme <https://w3id.org/gofairus/vocs/train1/idtype-grna> .

idtype:doi a skos:Concept;
  skos:prefLabel "DOI"@en;
  skos:definition "Digital Object Identifier; a character string used to uniquely identify an object. A DOI name is divided into two parts, a prefix and a suffix, separated by a slash."@en;
  skos:broader idtype:identifiertype;
  skos:inScheme <https://w3id.org/gofairus/vocs/train1/idtype-grna> .

idtype:ean13 a skos:Concept;
  skos:prefLabel "EAN13"@en;
  skos:definition "European Article Number, now renamed International Article Number, but retaining the original acronym, is a 13-digit barcoding standard which is a superset of the original 12-digit Universal Product Code (UPC) system."@en;
  skos:broader idtype:identifiertype;
  skos:inScheme <https://w3id.org/gofairus/vocs/train1/idtype-grna> .

idtype:eissn a skos:Concept;
  skos:prefLabel "EISSN"@en;
  skos:definition "Electronic International Standard Serial Number; ISSN used to identify periodicals in electronic form (eISSN or e- ISSN)."@en;
  skos:broader idtype:identifiertype;
  skos:inScheme <https://w3id.org/gofairus/vocs/train1/idtype-grna> .

idtype:handle a skos:Concept;
  skos:prefLabel "Handle"@en;
  skos:definition "A handle is an abstract reference to a resource."@en;
  skos:broader idtype:identifiertype;
  skos:inScheme <https://w3id.org/gofairus/vocs/train1/idtype-grna> .

idtype:igsn a skos:Concept;
  skos:prefLabel "IGSN"@en;
  skos:definition "International Geo Sample Number; a 9-digit alphanumeric code that uniquely identifies samples from our natural environment and related sampling features."@en;
  skos:broader idtype:identifiertype;
  skos:inScheme <https://w3id.org/gofairus/vocs/train1/idtype-grna> .

idtype:iri a skos:Concept;
  skos:prefLabel "IRI"@en;
  skos:definition "The Internationalized Resource Identifier (IRI) is an internet protocol standard which builds on the Uniform Resource Identifier (URI) protocol by greatly expanding the set of permitted characters."@en;
  skos:broader idtype:identifiertype;
  skos:narrower idtype:w3id;
  skos:inScheme <https://w3id.org/gofairus/vocs/train1/idtype-grna> .

idtype:isbn a skos:Concept;
  skos:prefLabel "ISBN"@en;
  skos:definition "International Standard Book Number; a unique numeric book identifier. There are 2 formats: a 10-digit ISBN format and a 13- digit ISBN."@en;
  skos:broader idtype:identifiertype;
  skos:inScheme <https://w3id.org/gofairus/vocs/train1/idtype-grna> .

idtype:issn a skos:Concept;
  skos:prefLabel "ISSN"@en;
  skos:definition "International Standard Serial Number; a unique 8-digit number used to identify a print or electronic periodical publication."@en;
  skos:broader idtype:identifiertype;
  skos:inScheme <https://w3id.org/gofairus/vocs/train1/idtype-grna> .

idtype:istc a skos:Concept;
  skos:prefLabel "ISTC"@en;
  skos:definition "International Standard Text Code; a unique number assigned to a textual work. An ISTC consists of 16 numbers and/or letters."@en;
  skos:broader idtype:identifiertype;
  skos:inScheme <https://w3id.org/gofairus/vocs/train1/idtype-grna> .

idtype:lissn a skos:Concept;
  skos:prefLabel "LISSN"@en;
  skos:definition "The linking ISSN or ISSN-L enables collocation or linking among different media versions of a continuing resource."@en;
  skos:broader idtype:identifiertype;
  skos:inScheme <https://w3id.org/gofairus/vocs/train1/idtype-grna> .

idtype:lsid a skos:Concept;
  skos:prefLabel "LSID"@en;
  skos:definition "Life Science Identifiers; a unique identifier for data in the Life Science domain. Format: urn:lsid:authority:namespace:id entifier:revision"@en;
  skos:broader idtype:identifiertype;
  skos:inScheme <https://w3id.org/gofairus/vocs/train1/idtype-grna> .

idtype:pmid a skos:Concept;
  skos:prefLabel "PMID"@en;
  skos:definition "PubMed identifier; a unique number assigned to each PubMed record."@en;
  skos:broader idtype:identifiertype;
  skos:inScheme <https://w3id.org/gofairus/vocs/train1/idtype-grna> .

idtype:purl a skos:Concept;
  skos:prefLabel "PURL"@en;
  skos:definition "Persistent Uniform Resource Locator. A PURL is an IRI, and therefore has three parts: (1) a protocol, (2) a resolver address, and (3) a name."@en;
  skos:broader idtype:identifiertype;
  skos:inScheme <https://w3id.org/gofairus/vocs/train1/idtype-grna> .

idtype:upc a skos:Concept;
  skos:prefLabel "UPC"@en;
  skos:definition "Universal Product Code is a barcode symbology used for tracking trade items in stores. Its most common form, the UPC-A, consists of 12 numerical digits."@en;
  skos:broader idtype:identifiertype;
  skos:inScheme <https://w3id.org/gofairus/vocs/train1/idtype-grna> .

idtype:uri a skos:Concept;
  skos:prefLabel "URI"@en;
  skos:definition "Uniform Resource Identifier is a string that provides a unique address (either on the Internet or on another private network, such as a computer filesystem or an Intranet) representing a resource, and implicitly describes where a resource can be found. A resource identification need not suggest the retrieval of resource representations over the Internet, nor need they imply network-based resources at all."@en;
  skos:broader idtype:identifiertype;
  skos:inScheme <https://w3id.org/gofairus/vocs/train1/idtype-grna> .

idtype:url a skos:Concept;
  skos:prefLabel "URL"@en;
  skos:definition "Uniform Resource Locator, also known as web address, is a specific character string that constitutes a reference to a resource. The syntax is: schema://domain:port/path?qu ery_string#fragment_id"@en;
  skos:broader idtype:identifiertype;
  skos:inScheme <https://w3id.org/gofairus/vocs/train1/idtype-grna> .

idtype:urn a skos:Concept;
  skos:prefLabel "URN"@en;
  skos:definition "Uniform Resource Name; is a unique and persistent identifier of an electronic document. The syntax is: urn:< NID>:<NSS> The leading urn: sequence is case-insensitive, <NID> is the namespace identifier, <NSS> is the namespace-specific string."@en;
  skos:broader idtype:identifiertype;
  skos:inScheme <https://w3id.org/gofairus/vocs/train1/idtype-grna> .

idtype:w3id a skos:Concept;
  skos:prefLabel "w3id"@en;
  skos:definition "Permanent identifier for Web applications. Mostly used to publish vocabularies and ontologies. The letters w3 stand for World Wide Web."@en;
  skos:broader idtype:iri;
  skos:inScheme <https://w3id.org/gofairus/vocs/train1/idtype-grna> .