@prefix schema: <http://schema.org/> .
@prefix pav: <http://purl.org/pav/> .
@prefix adms: <http://www.w3.org/ns/adms#> .
@prefix owl: <http://www.w3.org/2002/07/owl#> .
@prefix org: <http://www.w3.org/ns/org#> .
@prefix xls2rdf: <https://xls2rdf.sparna.fr/vocabulary#> .
@prefix xsd: <http://www.w3.org/2001/XMLSchema#> .
@prefix skosthes: <http://purl.org/iso25964/skos-thes#> .
@prefix rdfs: <http://www.w3.org/2000/01/rdf-schema#> .
@prefix qb: <http://purl.org/linked-data/cube#> .
@prefix assets: <https://w3id.org/gofairus/vocs/train1/digitalassets-yela/> .
@prefix dct: <http://purl.org/dc/terms/> .
@prefix rdf: <http://www.w3.org/1999/02/22-rdf-syntax-ns#> .
@prefix doap: <http://usefulinc.com/ns/doap#> .
@prefix sh: <http://www.w3.org/ns/shacl#> .
@prefix dcat: <http://www.w3.org/ns/dcat#> .
@prefix euvoc: <http://publications.europa.eu/ontology/euvoc#> .
@prefix prov: <http://www.w3.org/ns/prov#> .
@prefix foaf: <http://xmlns.com/foaf/0.1/> .
@prefix dc: <http://purl.org/dc/elements/1.1/> .
@prefix skos: <http://www.w3.org/2004/02/skos/core#> .
@prefix skosxl: <http://www.w3.org/2008/05/skos-xl#> .

<https://w3id.org/gofairus/vocs/train1/digitalassets-yela> a skos:ConceptScheme;
  dct:title "SKOS vocabulary for library's digital asset types for Yellow Team A";
  skos:prefLabel "SKOS vocabulary for library's digital asset types for Yellow Team A";
  dct:description "This is a template for building a SKOS-based controlled vocabulary. It is configured to support creation of a vocabulary by Yellow Team A.";
  foaf:homepage <https://github.com/fair-data-collective/excel2rdf-template>;
  dct:creator <https://orcid.org/0000-0001-6875-5360>, <https://orcid.org/0000-0003-2195-3997>,
    <https://orcid.org/0000-0002-9381-9693>;
  dct:contributor <https://orcid.org/0000-0001-8888-635X>;
  dct:rights <https://spdx.org/licenses/CC0-1.0>;
  owl:versionInfo "0.6.0";
  dct:created "2022-06-01T00:00:00+00:00"^^xsd:datetime;
  dct:modified "2025-06-08T15:49:00-07:00"^^xsd:datetime;
  skos:hasTopConcept assets:VeryTopConcept .

assets:VeryTopConcept a skos:Concept;
  skos:prefLabel "Very Top Concept"@en;
  skos:definition "In this vocabulary this Is a root concept for the whole vocabulary"@en;
  skos:altLabel "Root Concept";
  dct:creator <https://orcid.org/0000-0001-6875-5360>;
  skos:narrower assets:TopConceptOne, assets:TopConceptTwo;
  skos:inScheme <https://w3id.org/gofairus/vocs/train1/digitalassets-yela>;
  skos:topConceptOf <https://w3id.org/gofairus/vocs/train1/digitalassets-yela> .

assets:TopConceptOne a skos:Concept;
  skos:prefLabel "Top Concept One"@en;
  skos:definition "This is a top concept which is used to collect a number of narrower concepts."@en;
  skos:altLabel "Best Concept", "First Concept";
  skos:broader assets:VeryTopConcept;
  dct:creator <https://orcid.org/0000-0002-9381-9693>;
  dct:contributor <https://orcid.org/0000-0001-6875-5360>;
  skos:narrower assets:NarrowConceptOne, assets:NarrowConceptTwo;
  skos:inScheme <https://w3id.org/gofairus/vocs/train1/digitalassets-yela> .

assets:NarrowConceptOne a skos:Concept;
  skos:prefLabel "Narrow Concept One"@en;
  skos:definition "A definition of NarrowConceptOne, which has a broader concept TopConceptOne."@en;
  skos:broader assets:TopConceptOne;
  dct:creator <https://orcid.org/0000-0001-6875-5360>;
  skos:inScheme <https://w3id.org/gofairus/vocs/train1/digitalassets-yela> .

assets:NarrowConceptTwo a skos:Concept;
  skos:prefLabel "Narrow Concept Two"@en;
  skos:definition "A definition of NarrowConceptTwo, which has a broader concept TopConceptOne."@en;
  skos:broader assets:TopConceptOne;
  dct:creator <https://orcid.org/0000-0001-6875-5360>;
  skos:inScheme <https://w3id.org/gofairus/vocs/train1/digitalassets-yela> .

assets:TopConceptTwo a skos:Concept;
  skos:prefLabel "Top Concept Two"@en;
  skos:definition "This is yet another top concept which is used to collect a number of narrower concepts."@en;
  skos:altLabel "Second Concept", "Last Concept";
  skos:broader assets:VeryTopConcept;
  dct:creator <https://orcid.org/0000-0002-9381-9693>;
  dct:contributor <https://orcid.org/0000-0001-6875-5360>;
  skos:narrower assets:NarrowConceptThree, assets:NarrowConceptFour;
  skos:inScheme <https://w3id.org/gofairus/vocs/train1/digitalassets-yela> .

assets:NarrowConceptThree a skos:Concept;
  skos:prefLabel "Narrow Concept Three"@en;
  skos:definition "A definition of NarrowConceptThree, which has a broader concept TopConceptTwo."@en;
  skos:broader assets:TopConceptTwo;
  dct:creator <https://orcid.org/0000-0002-9381-9693>;
  dct:contributor <https://orcid.org/0000-0001-6875-5360>;
  skos:inScheme <https://w3id.org/gofairus/vocs/train1/digitalassets-yela> .

assets:NarrowConceptFour a skos:Concept;
  skos:prefLabel "Narrow Concept Four"@en;
  skos:definition "A definition of NarrowConceptFour, which has a broader concept TopConceptTwo."@en;
  skos:broader assets:TopConceptTwo;
  dct:creator <https://orcid.org/0000-0002-9381-9693>;
  dct:contributor <https://orcid.org/0000-0001-6875-5360>;
  skos:inScheme <https://w3id.org/gofairus/vocs/train1/digitalassets-yela> .